Start working on compositions of substitutions
This chunk supposes that substitutions sigma, tau are given by some
pair of lists. It then defines the correct list for their composition
and shows that the induced map agrees with the composotion on
variables.

It remains to show that it agrees on all terms, but this is the
obvious base case.

Term.v
@@ -3,6 +3,7 @@ Require Import Logic.Eqdep_dec.
 Require Import PeanoNat.
 Require Vectors.Fin.
 Require Vectors.VectorDef.
+Require Import Program.Basics.
 
 Require Import SymbComp.VecUtils.
 Require Import SymbComp.FinMod.
@@ -144,12 +145,52 @@ Section Term.
 
   Section comp_subst.
     Variables sigma tau : V -> Term.
+    Variable sl tl : list (V * Term).
+
     Hypothesis decV : forall x y : V, {x = y} + {x <> y}.
     Hypothesis decF : forall x y : F, {x = y} + {x <> y}.
 
-    (* TODO! *)
+    Hypothesis sH : forall v : V, sigma v = list_map decV varTerm sl v.
+    Hypothesis tH : forall v : V, tau v = list_map decV varTerm tl v.
 
-    (*Check (@fin_mod_is_list_map V decV Term varTerm
-                                (decTerm decV decF)).*)
+    (* A list inducing the correct correct composed map ([compose
+       sigma tau]) is given by first mapping all the variables to
+       where tau would send them and then applying the induced map
+       from sigma to the resulting term.
+
+       Variables that weren't moved by tau get mapped by sigma, which
+       we can express by shoving them to the end of the list.
+     *)
+    Local Definition stl : list (V * Term) :=
+      app (map (fun p => (fst p, subst_endo sigma (snd p))) tl)
+          sl.
+
+    Lemma stl_map_v (v : V)
+      : list_map decV varTerm stl v =
+        compose (subst_endo sigma) (subst_endo tau) (varTerm v).
+    Proof.
+      specialize (tH v).
+      unfold compose, subst_endo at 2, stl.
+      set (pmap := (fun p : V * Term => (fst p, subst_endo sigma (snd p)))).
+      revert tau tH.
+      induction tl as [ | p tl' IH ].
+      - intros; rewrite tH; clear tH; simpl; auto.
+      - intros tau tH.
+        clear tl; rename tl' into tl.
+        rewrite (map_cons pmap p tl), <- app_comm_cons.
+        destruct p as [ v' sv' ].
+        destruct (decV v' v) as [ veqH | vneH ].
+        + rewrite veqH in *; clear v' veqH.
+          simpl in tH; rewrite upd_map_at in tH.
+          unfold pmap; simpl; rewrite upd_map_at.
+          rewrite tH. tauto.
+        + unfold pmap at 1; simpl.
+          rewrite (upd_map_not_at decV _ _ (not_eq_sym vneH)).
+          simpl in tH.
+          rewrite (upd_map_not_at decV _ _ (not_eq_sym vneH)) in tH.
+          apply IH.
+          apply tH.
+    Qed.
+
   End comp_subst.
 End Term.
